make progress in writing spec

ironfleet/ravana/Node.i.dfy
@@ -11,7 +11,8 @@ module Protocol_Node_i {
 
   datatype Node =
       NodeLogger(
-          log: seq<LogEntry>
+          log: seq<LogEntry>,
+          clients: seq<EndPoint>
       )
     | NodeController(
           leader: bool,
@@ -20,24 +21,34 @@ module Protocol_Node_i {
 
           recved_events: map<SwitchIdPair, Event>,
 
-          log_copy: seq<LogEntry>
+          log_copy: seq<LogEntry>,
+          idx: int,
+
+          buffered_commands: map<int /* xid */, map<int /* command id */, SingleCommand>>,
+          current_command_id: int
       )
     | NodeSwitch(
           bufferedEvents: seq<Event>,
           switchState: SwitchState,
           event_id: int,
-          master: EndPoint
+          master: EndPoint,
+          received_command_ids: seq<int>
       )
 
   predicate NodeInit(node: Node, my_index: int, config: Config) {
     (
       node.NodeLogger? &&
-        node.log == []
+        node.log == [] &&
+        node.clients == config.node_controllers
     ) || (
       node.NodeController? &&
         node.leader == (my_index == 0) &&
         controllerStateInit(node.controllerState) &&
-        node.config == config
+        node.config == config &&
+        node.recved_events == map[] &&
+        node.log_copy == [] &&
+        node.current_command_id == 0 &&
+        node.idx == 0
     ) || (
       node.NodeSwitch? &&
         node.bufferedEvents == [] &&
@@ -60,24 +71,155 @@ module Protocol_Node_i {
        && packet.dst == s.master
   }
 
-  predicate Node_ControllerLogEvent(s: Node, s': Node, ios: seq<RavanaIo>) {
+  // TODO I think we want to combine these two:
+
+  predicate Node_ControllerRecvEvent(s: Node, s': Node, ios: seq<RavanaIo>) {
     s.NodeController? &&
     s.leader &&
-    s' == s &&
-    |ios| == 2 &&
+
+    |ios| == 1 &&
     ios[0].LIoOpReceive? &&
-    ios[1].LIoOpSend? &&
     var recv_packet := ios[0].r;
-    var send_packet := ios[1].s;
 
     recv_packet.msg.EventMessage? &&
 
-    send_packet.dst == s.config.node_logger &&
-    send_packet.msg == LogMessage(LMRecv(
-        recv_packet.src, recv_packet.msg.event, recv_packet.msg.event_id))
+    s' == s.(recved_events := s.recved_events[
+        SwitchIdPair(recv_packet.src, recv_packet.msg.event_id) := recv_packet.msg.event])
   }
 
-  // TODO get the log 
+  predicate Node_ControllerLogEvent(s: Node, s': Node, p: SwitchIdPair, ios: seq<RavanaIo>) {
+    s.NodeController? &&
+    s.leader &&
 
-  //predicate Node_ControllerProc
+    p in s.recved_events &&
+
+    |ios| == 1 &&
+    ios[0].LIoOpSend? &&
+    var send_packet := ios[0].s;
+    send_packet.dst == s.config.node_logger &&
+    send_packet.msg == LogMessage(LMRecv(p.switch, s.recved_events[p], p.event_id))
+  }
+
+  predicate Node_LoggerLogEvent(s: Node, s': Node, ios: seq<RavanaIo>) {
+    s.NodeLogger? &&
+
+    |ios| == 1 &&
+    ios[0].LIoOpReceive? &&
+    var recv_packet := ios[0].r;
+    recv_packet.msg.LogMessage? &&
+
+    s' == s.(log := s.log + [recv_packet.msg.log_entry])
+  }
+
+  predicate Node_LoggerBroadcast(s: Node, s': Node, ios: seq<RavanaIo>) {
+    s.NodeLogger? &&
+    s' == s &&
+
+    |ios| == |s.clients| &&
+    forall i :: 0 <= i < |s.clients| ==>
+        ios[i].LIoOpSend? &&
+        ios[i].s.dst == s.clients[i] &&
+        ios[i].s.msg == LogBroadcastMessage(s.log)
+  }
+
+  predicate Node_ControllerReadLog(s: Node, s': Node, ios: seq<RavanaIo>) {
+    s.NodeController? &&
+    |ios| == 1 &&
+    ios[0].LIoOpReceive? &&
+    var recv_packet := ios[0].r;
+    recv_packet.src == s.config.node_logger &&
+    recv_packet.msg.LogBroadcastMessage? &&
+    var new_log_copy := recv_packet.msg.full_log;
+    s' == s.(log_copy :=
+        if |new_log_copy| > |s.log_copy| then new_log_copy else s.log_copy)
+  }
+
+  predicate Node_ControllerProcessEntry(s: Node, s': Node, ios: seq<RavanaIo>) {
+    // TODO there should be something that checks if it's the leader, here
+    // TODO should send EventAck to the client
+    s.NodeController? &&
+    0 <= s.idx < |s.log_copy| &&
+    ios == [] &&
+    var l := s.log_copy[s.idx];
+    (
+      l.LMRecv? &&
+      var (new_state, commands) := controllerTransition(s.controllerState, l.switch, l.event);
+      (
+        // Leader: prepare commands to send to switches
+        s.leader &&
+        var new_bc :=
+            map i : int
+                  | s.current_command_id <= i < s.current_command_id + |commands|
+                 :: commands[i - s.current_command_id];
+        s' == s.
+            (idx := s.idx + 1).
+            (current_command_id := s.current_command_id + |commands|).
+            (controllerState := new_state).
+            (buffered_commands := s.buffered_commands[s.idx := new_bc])
+      ) || (
+        // Slave: 
+        !s.leader &&
+        (exists j : int :: 0 <= j < |s.log_copy| && s.log_copy[j] == LMProc(s.idx)) &&
+        s' == s.
+            (idx := s.idx + 1).
+            (controllerState := new_state).
+            (current_command_id := s.current_command_id + |commands|)
+      )
+    ) || (
+      l.LMProc? &&
+      s' == s.(idx := s.idx + 1)
+    )
+  }
+
+  predicate Node_ControllerSendCommand(
+      s: Node, s': Node, xid: int, command_id: int, ios: seq<RavanaIo>) {
+    s.NodeController? &&
+    s.leader &&
+    xid in s.buffered_commands &&
+    command_id in s.buffered_commands[xid] &&
+    var comm := s.buffered_commands[xid][command_id];
+    |ios| == 1 &&
+    ios[0].LIoOpSend? &&
+    var send_packet := ios[0].s;
+    send_packet.dst == comm.switch &&
+    send_packet.msg == CommandMessage(comm.command, command_id)
+  }
+
+  predicate Node_SwitchRecvCommand(
+      s: Node, s': Node, ios: seq<RavanaIo>) {
+    s.NodeSwitch? &&
+    |ios| >= 1 &&
+    ios[0].LIoOpReceive? &&
+    var recv_packet := ios[0].r;
+    recv_packet.msg.CommandMessage? &&
+    var command := recv_packet.msg.command;
+    var command_id := recv_packet.msg.command_id;
+    (
+      // not from the master: just ignore it
+      recv_packet.src != s.master &&
+      |ios| == 1 &&
+      s' == s
+    ) ||
+    (
+      // from the master
+      recv_packet.src == s.master &&
+
+      // send an ACK in any case
+      |ios| == 2 &&
+      ios[1].LIoOpSend? &&
+      var send_packet := ios[1].s;
+      send_packet.msg == CommandAck(command_id) &&
+
+      ((
+        // already got this one, don't do anything else
+        (command_id in s.received_command_ids) &&
+        s' == s
+      ) || (
+        // apply to state, save the command_id
+        !(command_id in s.received_command_ids) &&
+        s' == s.(received_command_ids := s.received_command_ids + [command_id])
+               .(switchState := switchTransition(s.switchState, command))
+      ))
+    )
+  }
 }
